Veritas.Verifier.Blum.fsti
@@ -10,7 +10,8 @@ open Veritas.Verifier
 open Veritas.Verifier.CorrectDefs
 open Veritas.Verifier.TSLog
 
-module M=Veritas.MultiSetHash
+module MS=Veritas.MultiSet
+module MH=Veritas.MultiSetHash
 module TL=Veritas.Verifier.TSLog
 
 (* global add sequence *)
@@ -74,12 +75,26 @@ let ts_add_set_key (#n:pos) (itsl: its_log n) (k:key): mset ms_hashfn_dom
 val lemma_ts_add_set_correct (#n:pos) (itsl: its_log n): 
   Lemma (ts_add_set itsl == g_add_set (partition_idx_seq itsl))
 
+(* if the tail element is a blum add, then the add set is obtained by adding that 
+ * blum add to the prefix *)
+val lemma_ts_add_set_key_extend (#n:pos) (itsl: its_log n {length itsl > 0}):
+  Lemma (requires (is_blum_add (telem itsl)))
+        (ensures (ts_add_set_key itsl (key_of itsl (length itsl - 1)) == 
+                  add_elem (ts_add_set_key (its_prefix itsl (length itsl - 1))
+                                           (key_of itsl (length itsl - 1)))
+                           (blum_add_elem (telem itsl))))
+
 (* is the index i of ts log an blum evict *)
-val is_blum_evict (#p:pos) (itsl: its_log p) (i: seq_index itsl): bool
+let is_blum_evict (#n:pos) (itsl: its_log n) (i: seq_index itsl): bool = 
+  let (e,_) = index itsl i in
+  match e with
+  | EvictB _ _ -> true
+  | EvictBM _ _ _ -> true
+  | _ -> false
 
 (* get the blum evict element from an index *)
 val blum_evict_elem (#p:pos) (itsl: its_log p) (i:seq_index itsl{is_blum_evict itsl i}):
-  (e:ms_hashfn_dom{M.key_of e = TL.key_of itsl i})
+  (e:ms_hashfn_dom{MH.key_of e = TL.key_of itsl i})
 
 (* sequence of evicts in time sequence log *)
 val ts_evict_seq (#n:pos) (itsl: its_log n): seq ms_hashfn_dom
@@ -98,6 +113,15 @@ let ts_evict_set_key (#n:pos) (itsl: its_log n) (k:key): mset ms_hashfn_dom=
 val lemma_ts_evict_set_correct (#n:pos) (itsl: its_log n):
   Lemma (ts_evict_set itsl == g_evict_set (partition_idx_seq itsl))
 
+(* if the tail element is not an evict, the evict set is the same as the evict 
+ * set of the length - 1 prefix 
+ *)
+val lemma_ts_evict_set_key_extend2 (#n:pos) (itsl: its_log n {length itsl > 0}):
+  Lemma (requires (not (is_blum_evict itsl (length itsl - 1))))
+        (ensures (ts_evict_set_key itsl (key_of itsl (length itsl - 1)) == 
+                  ts_evict_set_key (its_prefix itsl (length itsl - 1))
+                                           (key_of itsl (length itsl - 1))))
+
 (* since evict_set is a pure set (not a multiset) we can identify the unique index 
  * for each element of the set *)
 val index_blum_evict (#p:pos) (itsl: its_log p) (e: ms_hashfn_dom {contains e (ts_evict_set itsl)}):
@@ -109,4 +133,27 @@ val lemma_evict_before_add (#p:pos) (itsl: its_log p) (i:seq_index itsl{is_blum_
   Lemma (requires True)
         (ensures (not (contains (blum_add_elem (index itsl i)) (ts_evict_set itsl)) \/
                   index_blum_evict itsl (blum_add_elem (index itsl i)) < i))
-         
+
+(* a slightly different version of of the previous lemma - the count of an add element 
+ * in the evict set is the same in the prefix as the full sequence *)
+val lemma_evict_before_add2 (#p:pos) (itsl: its_log p) (i:seq_index itsl{is_blum_add (index itsl i)}):
+   Lemma (requires True)
+         (ensures (MS.mem (blum_add_elem (index itsl i)) (ts_evict_set itsl) =
+                   MS.mem (blum_add_elem (index itsl i)) (ts_evict_set (its_prefix itsl i))))
+
+(* for an eac ts log, if the eac state of a key k is instore, the count of blum evicts 
+ * is the same of blum adds for that key *)
+val lemma_evict_add_count_same (#p:pos) (itsl: eac_ts_log p) (k:key):
+  Lemma (requires (is_eac_state_instore itsl k))
+        (ensures (MS.size (ts_add_set_key itsl k) = MS.size (ts_evict_set_key itsl k)))
+
+val lemma_mem_key_add_set_same (#p:pos) (itsl: eac_ts_log p) (be: ms_hashfn_dom):
+  Lemma (mem be (ts_add_set itsl) = mem be (ts_add_set_key itsl (MH.key_of be)))
+
+val lemma_mem_key_evict_set_same (#p:pos) (itsl: eac_ts_log p) (be: ms_hashfn_dom):
+  Lemma (mem be (ts_evict_set itsl) = mem be (ts_evict_set_key itsl (MH.key_of be)))
+
+(* the count of an element can only decrease in a prefix of itsl *)
+val lemma_mem_monotonic (#p:pos) (be:ms_hashfn_dom) (itsl: eac_ts_log p) (i:nat{i < length itsl}):
+  Lemma (mem be (ts_evict_set itsl) >= mem be (ts_evict_set (its_prefix itsl i)) /\
+         mem be (ts_add_set itsl) >= mem be (ts_add_set (its_prefix itsl i)))
